Add channel iteration and collection into slice ex

go/iterator/channel_iter.go
@@ -1,0 +1,28 @@
+package iterator
+
+func chanIter[V any](channel <-chan V) func(yield func(V) bool) {
+	return func(yield func(V) bool) {
+		// TODO: should channel closure be deferred?
+		for v := range channel {
+			if !yield(v) {
+				return
+			}
+		}
+	}
+}
+
+func collectChannel[V any](channel <-chan V) []V {
+	s := make([]V, 0 /* random number */)
+
+	loop_body := func(v V) bool {
+		s = append(s, v)
+
+		return true
+	}
+
+	iterator := chanIter[V](channel)
+
+	iterator(loop_body)
+
+	return s
+}
