src/iter/chan_iter.v
@@ -1,0 +1,185 @@
+From sys_verif.program_proof Require Import prelude empty_ffi.
+From New.proof Require Import std.
+From New.generatedproof.sys_verif_code Require Import iterator.
+From New.proof.github_com.goose_lang.goose.model.channel
+  Require Import chan_au_base.
+From New.proof.github_com.goose_lang.goose.model.channel.protocol
+     Require Import base simple future spsc done dsp (* dsp_proofmode *) mpmc join handshake.
+From New.golang.theory Require Import chan.
+
+Section proof.
+Context `{hG: !heapGS Σ} `{!globalsGS Σ} {go_ctx: GoContext}.
+
+Context `{!IntoVal V} `{!IntoValTyped V vt}.
+Context `{!chanG Σ V}.
+
+#[global] Instance : IsPkgInit iterator := define_is_pkg_init True%I.
+#[global] Instance : GetIsPkgInitWf iterator := build_get_is_pkg_init_wf.
+
+Definition is_chanIter (chanIter : func.t) : iPropI Σ :=
+  ∀ (Inv : iPropI Σ) (P : V → iPropI Σ) (Φ : iPropI Σ) (yield : func.t), (
+    "Hinv" :: Inv ∗
+    "#Hyield" :: □(
+      ∀ (v : V),
+      Inv ∗ P(v) -∗
+      WP #yield #v {{
+        ok,
+        if (decide (ok = #true)) then
+          Inv
+        else if (decide (ok = #false)) then
+          Φ
+        else
+          False
+      }}
+    )∗
+    "Htrace" (* TODO: misleading name *) :: (Inv -∗ Φ)
+  )%I -∗
+  WP #chanIter #yield {{ _, Φ }}.
+
+Lemma wp_chanIter (ch : loc) (γ : chan_names) :
+  {{{
+    is_pkg_init iterator ∗
+    "His_channel" :: is_channel ch γ ∗
+    "Hown_channel" :: own_channel ch chan_rep.Idle γ
+  }}}
+    @! iterator.chanIter #vt #ch
+  {{{ (f : func.t), RET #f; is_chanIter f }}}.
+Proof.
+  wp_start. iNamed "Hpre".
+  wp_auto.
+  iApply "HΦ".
+  clear Φ.
+  unfold is_chanIter.
+  iIntros (? ? ? ?) "Hpre".
+  iNamed "Hpre".
+  wp_auto.
+  unfold chan.for_range.
+  wp_auto.
+  (* TODO: clean this up :( )*)
+  iPoseProof (start_simple ch γ P) as "Hsimple".
+  iApply "Hsimple" in "His_channel".
+  iApply "His_channel" in "Hown_channel".
+  iMod "Hown_channel" as (γsimple) "[%Heq #His_simple]".
+  iAssert (
+    ∃(v : V),
+    "Hinv" :: Inv ∗
+    "v" :: v_ptr ↦ v
+  )%I with "[Hinv v]" as "Hinv2" ; first iFrame.
+  wp_for "Hinv2".
+  wp_apply (wp_simple_receive with "[His_simple]") ; first done.
+  iIntros (?) "HP".
+  wp_auto.
+  wp_bind (#yield _).
+  iApply (wp_wand with "[Hinv HP]").
+  {
+    iApply "Hyield".
+    iFrame.
+  }
+  iIntros (ok) "Hok".
+  destruct (decide _).
+  {
+    subst.
+    wp_auto.
+    wp_for_post.
+    iFrame.
+  }
+  destruct (decide _).
+  {
+    subst.
+    wp_auto.
+    wp_for_post.
+    done.
+  }
+  done.
+Qed.
+
+Lemma wp_collectChannel (ch : loc) (γ : chan_names) (P : V → iPropI Σ) :
+  {{{
+    is_pkg_init iterator ∗
+    "His_channel" :: is_channel ch γ ∗
+    "Hown_channel" :: own_channel ch chan_rep.Idle γ
+  }}}
+    @! iterator.collectChannel #vt #ch
+  {{{ 
+    (s : slice.t), RET #s; 
+    ∃ (trace : list V), own_slice s 1 trace ∗
+    ([∗ list] k ↦ x ∈ trace, P x)
+  }}}.
+Proof.
+  wp_start. iNamed "Hpre".
+  wp_auto.
+  wp_apply wp_slice_make2 ; first word.
+  iIntros (?) "[Hsl Hsl_cap]".
+  replace (sint.nat (W64 0)) with 0%nat by word.
+  rewrite replicate_0.
+  set (l := []).
+  wp_auto.
+  wp_apply (wp_chanIter with "[His_channel Hown_channel]") ; first iFrame.
+  iIntros (?) "His_chanIter".
+  wp_auto.
+  unfold is_chanIter.
+  wp_bind (#f _).
+  iApply (wp_wand with "[s Hsl Hsl_cap His_chanIter]").
+  {
+    set Inv := (
+      ∃ l trace, 
+      "Htrace" :: ([∗ list] k ↦ x ∈ trace, P x) ∗ 
+      "s" :: s_ptr ↦ l ∗
+      "Hsl" :: l ↦* trace ∗
+      "Hsl_cap" :: own_slice_cap V l (DfracOwn 1)
+    )%I.
+    wp_apply (
+      "His_chanIter" $!
+      Inv
+      P
+      Inv
+    ).
+    iSplitL "s Hsl Hsl_cap".
+    {
+      iExists sl.
+      iExists [].
+      subst l.
+      iFrame.
+      rewrite big_sepL_nil.
+      done.
+    }
+    iSplitR.
+    {
+      iModIntro.
+      iIntros (v) "[Hinv HP]".
+      iNamed "Hinv".
+      wp_auto.
+      wp_apply wp_slice_literal.
+      iIntros (lv) "Hlv".
+      wp_auto.
+      wp_apply (wp_slice_append with "[Hsl Hsl_cap Hlv]"); first iFrame.
+      iIntros (?) "[Hs' [Hs'_cap Hlv]]".
+      wp_auto.
+      destruct (decide _).
+      2: {
+        iExFalso.
+        iPureIntro.
+        apply n.
+        done.
+      }
+      iExists s'.
+      iExists (trace0 ++ [v]).
+      iFrame.
+      rewrite big_sepL_nil.
+      done.
+    }
+    iIntros "Hinv".
+    iNamed "Hinv".
+    iExists l0.
+    iExists trace0.
+    iFrame.
+  }
+  iIntros (v) "Hinv".
+  iNamed "Hinv".
+  wp_auto.
+  iApply "HΦ".
+  iExists trace0.
+  iFrame.
+Qed.
+
+End proof.
